noc/NOC_setup.v
@@ -1,6 +1,9 @@
 Require Import Koika.Frontend.
 Require Import Koika.Std.
-Require Import Koika.Testing.
+Require Import Router.
+Require Import Types.
+From Coq Require Import Arith Lia Program.
+From Equations Require Import Equations.
 
 Module Type NOC_data.
   Parameter nocsize: nat.
@@ -12,12 +15,95 @@ Import Types.
 Definition regno := (Nat.sub nocsize 1).
 
 Inductive reg_t := reg_ (n: Vect.index regno).
-Inductive rule_name_t := router_ (n: Vect.index nocsize).
+Inductive rule_name_t :=
+  | route0_r
+  | route1_r
+  | route2_r
+  | route3_r.
+
+(* Inductive rule_name_t := router_ (n: Vect.index nocsize). *)
+
+  (* Axiom index_of_nat_never_none : forall n, index_of_nat regno n <> None. 
+Equations reg (n : nat) : reg_t :=  
+  reg n :=
+  match index_of_nat regno n with
+  | Some m => reg_ m
+  | None => absurd (index_of_nat regno n = None) index_of_nat_never_none 
+  end. *)
+(* 
+ Definition router n :=
+  router_ (match index_of_nat nocsize n with
+        | Some n => n
+        | None => thisone
+        end).  
+  *)
+Module MyRegs <: Registers.
+  Definition reg_t:=reg_t.
+End MyRegs.
 
 
-Definition routefail(r_addr2: nat) (r0: reg_t) 
-: uaction reg_t empty_ext_fn_t :=
-{{ fail }}.
+Module Routerfns:= Router(MyRegs).        
+Import Routerfns.
+Compute index 3.
+Compute index_of_nat nocsize 1.
+
+
+Fixpoint list_seq_index_anotherone {N : nat} (l : list (index N)) : list (index (S N)) :=
+  match l with
+  | nil => nil
+  | cons el l' => cons (anotherone el) (list_seq_index_anotherone l')
+  end.
+
+(* Constucting an ascending list of all possible indecies N *)
+Fixpoint list_seq_index (N : nat) : list (index N) :=
+  match N with
+  | O => nil
+  | S N' => cons (thisone) (list_seq_index_anotherone (list_seq_index N'))
+  end.
+
+  Fixpoint get_nth_item_default {A : Type} (l : list A) (n : nat) (default : A) : A :=
+    match l, n with
+    | [], _ => default
+    | x :: _, 0 => x
+    | _ :: xs, S n' => get_nth_item_default xs n' default
+    end.
+  
+(* Fixpoint get_nth_item_fin {A : Type} (l : list A) (n : Fin.t regno) : A :=
+  match l with
+  | [] => match n with end (* This case is impossible due to the dependent type *)
+  | x :: xs =>
+    match n with
+    | Fin.F1 => x
+    | Fin.FS n' => get_nth_item_fin xs n'
+    end
+  end. *)
+
+
+Definition indices := list_seq_index regno.
+Compute indices.
+Check get_nth_item_default indices 1.
+(* Definition get_reg (n: nat): reg_t := reg_ (get_nth_item_default indices n). *)
+
+(* Fixpoint give_index (n: nat) : index nocsize :=
+  match n with
+  | 0 => thisone
+  | S n' => anotherone (give_index n')
+  end. *)
+
+(* Equations to_action (rl : rule_name_t) : uaction reg_t empty_ext_fn_t := 
+to_action (router_ idx) :=
+  let idx_nat := index_to_nat idx in
+  if Nat.eqb idx_nat 0 then
+    routestartfn 0 (reg_ get_nth_item_default indices 1)
+  else if Nat.eqb idx_nat regno then
+    let idx' := index_of_nat (Nat.sub idx_nat - 1) in
+    routeendfn regno (reg_ idx')
+  else
+    let idx' := index_of_nat (Nat.sub idx_nat - 1) in
+    routecenterfn idx_nat (reg_ idx') (reg_ idx). *)
+
+
+
 
 
 End NOCSetup.
